\documentclass{ben}
\title{MATH 112A Homework 3}
\author{Benjamin Tong}
\date{October 31, 2025}

\begin{document}
\maketitle
\section{Monday}
\subsection{Problem 1}
Solve
\[
    u_{xx} + 3 u_{xt} - 4 u_{tt} = 0,\ u(x, 0) = \sin x,\ u_t(x, 0) = \frac{1}{1 + x^2}
\]
\begin{solution}
First, we rewrite the function and factor. We get
\begin{align*}
    \left( \frac{\partial^2}{\partial x^2}
    + 3 \frac{\partial^2}{\partial x \partial t}
    - 4 \frac{\partial^2}{\partial t^2} \right) u &= 0\\
    \left( \partials{x} + 4 \partials{t} \right)
    \underbrace{\left( \partials{x} - \partials{t} \right) u}_{v} &= 0\\
    \left( \partials{x} + 4 \partials{t} \right) v &= 0\\
    v_x + 4 v_t &= 0\\
    v &= f(4x - t)
\end{align*}
Now, we resubstitute in $v = \left( \partials{x} - \partials{t} \right) u$ and we get
\begin{align*}
    \left( \partials(x) - \partials{t} \right) u &= f(4x - t)\\
    u_x - u_t &= f(4x - t)
\end{align*}
We use the change of coordinates $x' = x - t$ and $t' = x + t$, and we get
\begin{align*}
    u_x - u_t &= f(4x - t)\\
    (u_{x'} + u_{t'}) - (-u_{x'} + u_{t'})
    &= f\left(4\left(\frac{1}{2}x' + \frac{1}{2}t'\right) - \left(-\frac{1}{2}x' - \frac{1}{2}t'\right)\right)\\
    2 u_{x'} &= f\left( 2x' + 2t' - \frac{1}{2}x' + \frac{1}{2}t' \right)\\
    2 u_{x'} &= f\left(\frac{3}{2} x' + \frac{5}{2} t'\right)\\
    u_{x'} &= \frac{1}{2} f \left( \frac{3}{2} x' + \frac{5}{2} t' \right)\\
    u &= \frac{1}{3} F \left( \frac{3}{2} x' + \frac{5}{2} t' \right) + G(t')\\
    u &= \frac{1}{3} F \left(4x - t\right) + G(x + t)\\
\end{align*}
where $F$ and $G$ are the anti-derivatives of $f$ and $g$.
We also find that
\[
    u_t = -\frac{1}{3} f(4x - t) + g(x + t)
\]
If we substitute $t = 0$ we find that
\begin{align*}
    u(x, 0) &= \frac{1}{3} F(4x) + G(x)\\
    \sin x &= \frac{1}{3}F(4x) + G(x)\\
\end{align*}
Differentiating this we get $\cos x = \frac{4}{3}f(4x) + g(x)$.
Now, if we substitute $t = 0$ into $u_t(x, t)$ we get
\begin{align*}
    u_t(x, 0) &= -\frac{1}{3} f(4x) + g(x)\\
    \frac{1}{1 + x^2} &= -\frac{1}{3} f(4x) + g(x)\\
\end{align*}
So now we have the equations
\begin{align*}
    \cos x &= \frac{4}{3}f(4x) + g(x)\\
    \frac{1}{1 + x^2} &= -\frac{1}{3} f(4x) + g(x)
\end{align*}
From this we find that
\begin{align*}
    f(x) &= \frac{3}{5} \left( \cos \frac{x}{4} - \frac{1}{1 + \frac{x^2}{16}} \right)\\
    g(x) &= \frac{1}{5} \left( \cos x + \frac{4}{1 + x^2} \right)
\end{align*}
We find that the anti-derivatives of these functions are
\begin{align*}
    F(x) &= \frac{3}{5} \left( 4 \sin \left( \frac{x}{4} \right)
    - 4 \arctan \left( \frac{x}{4} \right) \right) + C\\
    G(x) &= \frac{1}{5} \left( \sin(x) + 4 \arctan(x) \right) + C
\end{align*}
and so we finally get that
\begin{align*}
    u(x, t) &= \frac{1}{3} F(4x - t) + G(x + t)\\
    &= \frac{1}{3} \left( \frac{3}{5} \left( 4 \sin \left( \frac{4x - t}{4} \right)
    - 4 \arctan \left( \frac{4x - t}{4} \right) \right) \right)
    + \left( \frac{1}{5} \left( \cos (x + t) + 4 \arctan(x + t) \right) \right)\\
    &= \frac{4}{5} \sin\left( \frac{4x - t}{4} \right) - 4 \arctan \left( \frac{4x - t}{4} \right)
    + \frac{1}{5} \cos (x + t) + \frac{4}{5} \arctan(x + t)
\end{align*}
\end{solution}
\newpage
\section{Wednesday}
\subsection{Problem 1}
Solve the following initial value problem.
\[
\begin{cases}
    u_{xx} - 3u_{xt} - 4u_{tt} = 1, & -\infty < x < \infty, 0 < t < \infty\\
    u(x, 0) = x^2, & -\infty < x < \infty\\
    u_t(x, 0) = e^x, & -\infty < x < \infty
\end{cases}
\]
\begin{solution}
  We find that the differential equation is equal to
  \[
    \left( \partials{x} - 4 \partials{t} \right) \left( \partials{x} + \partials{t} \right)u = 1
  \]
  We can define $v = \left( \partials{x} + \partials{t} \right)u$, and we get the system
  \begin{align*}
    \left( \partials{x} - 4 \partials{t} \right)v &= 1\\
    \left( \partials{x} + \partials{t} \right)u = v
  \end{align*}
  First, we solve for $v$. We find that
  \[
    \frac{dx}{1} = \frac{dt}{4} = \frac{dv}{1}
  \]
  and so
  \begin{align*}
    \frac{dx}{dt} &= \frac{-1}{4}\\
    x &= -\frac{1}{4}t + \xi
  \end{align*}
  so the characteristic curves are where $\xi = x + \frac{1}{4}t$ remains constant.
  Now, we also find that
  \begin{align*}
    \frac{dv}{dx} &= 1\\
    v &= x + f(\xi)\\
    v &= x + f \left( x + \frac{1}{4}t \right)
  \end{align*}
  Now, we solve for $u$. We find that
  \[
    \frac{dx}{1} = \frac{dt}{1} = \frac{du}{x + f \left( x + \frac{1}{4}t \right)}
  \]
  and so
  \begin{align*}
    \frac{dx}{dt} &= 1\\
    x &= t + \eta\\
  \end{align*}
  and so the characteristic curves are where $\eta = x - t$ remains constant.
  Now, we also find that
  \[
    \frac{du}{dx} = x + f \left( x + \frac{1}{4}t \right)
  \]
  We use the substitution $t = x - \eta$ in order to rewrite this expression in terms of $x$ and
  $\eta$. Doing this, we get
  \begin{align*}
    \frac{du}{dx} &= x + f \left( x + \frac{1}{4}(x - \eta) \right)\\
                  &= x + f \left( \frac{5}{4}x - \frac{1}{4}\eta \right)
  \end{align*}
  Integrating this on both sides, and using the substitution $\eta = x - t$ we get that
  \begin{align*}
    u &= \frac{1}{2} x^2 + \frac{4}{5} F \left( \frac{5}{4} x - \frac{1}{4} \eta \right) + G(\eta)\\
      &= \frac{1}{2} x^2 + \frac{4}{5} F \left( x + \frac{1}{4}t \right) + G(x - t)
  \end{align*}
\end{solution}
\section{Friday}
\subsection{Problem 1}
For a solution $u(x, t)$ of the wave equation with $\rho = T = c = 1$, the energy density is defined
as
\[
    e = \frac{1}{2} \left( u_t^2 + u_x^2 \right)
\]
and the momentum density as
\[
    p = u_t u_x
\]
Show that
\begin{enumerate}
    \item $\partials[e]{t} = \partials[p]{x}$ and $\partials[p]{t} = \partials[e]{x}$.
    \item Show that both $e(x, t)$ and $p(x, t)$ also satisfy the wave equation.
\end{enumerate}
\subsection{Problem 2}
For a wave equation, if significant air resistance $r > 0$ is present, we have an extra term
proportional to the speed $u_t$, thus the equation becomes
\[
    u_{tt} - c^2 u_{xx} + r u_t = 0
\]
Show that the energy decreases.
\end{document}
